examples/map/MapMAproof.v
@@ -35,16 +35,16 @@ Section SIMMODSEM.
   Let W: Type := Any.t * Any.t.
 
   Definition initial_map: iProp :=
-    OwnM (Excl.unit, Auth.excl ((fun _ => Excl.just 0%Z): @URA.car (nat ==> (Excl.t Z))%ra) ((fun _ => Excl.just 0%Z): @URA.car (nat ==> (Excl.t Z))%ra)).
+    OwnM (Excl.unit, Auth.excl ((fun _ => Excl.just 0%Z): @URA.car (Z ==> (Excl.t Z))%ra) ((fun _ => Excl.just 0%Z): @URA.car (Z ==> (Excl.t Z))%ra)).
 
   Definition black_map (f: Z -> Z): iProp :=
-    OwnM (Excl.unit, Auth.black ((fun k => Excl.just (f k)): @URA.car (nat ==> (Excl.t Z))%ra)).
+    OwnM (Excl.unit, Auth.black ((fun k => Excl.just (f k)): @URA.car (Z ==> (Excl.t Z))%ra)).
 
   Definition unallocated (sz: Z): iProp :=
     OwnM (Excl.unit, Auth.white ((fun k =>
                                     if (Z_gt_le_dec 0 k) then Excl.just 0%Z
                                     else if (Z_gt_le_dec sz k) then Excl.unit else Excl.just 0%Z)
-                                  : @URA.car (nat ==> (Excl.t Z))%ra)).
+                                  : @URA.car (Z ==> (Excl.t Z))%ra)).
 
   Lemma initial_map_initialize sz
     :
@@ -66,7 +66,7 @@ Section SIMMODSEM.
 
   Lemma black_map_get f k v
     :
-    black_map f -∗ map_points_to k v -∗ (black_map f ** map_points_to k v ** (⌜f k = v⌝)).
+    black_map f -∗ map_points_to k v -∗ (⌜f k = v⌝).
   Proof.
   Admitted.
 
@@ -80,7 +80,7 @@ Section SIMMODSEM.
         @mk_wf
           _ unit
           (fun _ st_src st_tgt =>
-             ((∃ f sz, ⌜st_src = f↑ /\ st_tgt = (f, sz)↑⌝ ** black_map f ** unallocated sz ** pending1) ∨ (initial_map))%I).
+             ((∃ f sz, ⌜st_src = f↑ /\ st_tgt = (f, sz)↑⌝ ** black_map f ** unallocated sz ** pending1) ∨ (initial_map ** ⌜st_src = (fun (_: Z) => 0%Z)↑ /\ st_tgt = (fun (_: Z) => 0%Z, 0%Z)↑⌝))%I).
 
   Variable GlobalStbM: Sk.t -> gname -> option fspec.
   Hypothesis STB_setM: forall sk, (GlobalStbM sk) "set" = Some set_specM.
@@ -104,403 +104,177 @@ Section SIMMODSEM.
     eapply adequacy_local2. econs; ss.
     i. econstructor 1 with (wf:=wf) (le:=top2); ss.
     2: { esplits. econs; et. eapply to_semantic. iIntros "H". iSplitL "H"; eauto. iApply Own_unit. ss. }
-    Local Opaque black_map map_points_to unallocated.
+    Local Opaque initial_map black_map map_points_to unallocated.
     econs.
-    { admit "". }
-
-    econs; ss.
-
     {
       init.
       rename mp_tgt into mpr_tgt.
       assert(exists mp_src mp_tgt (mr_src mr_tgt: Σ),
                 mrp_src = Any.pair mp_src mr_src↑ ∧ mpr_tgt = Any.pair mp_tgt mr_tgt↑).
       { inv WF. esplits; et. } des; clarify.
-      (*** get ***)
+      (*** init ***)
+      unfold MapM.initF, MapA.initF, ccallU, ccallN.
+      harg. fold wf. ss.
+      unfold pending in ACC. mDesAll; des; clarify.
+      mDesOr "INVS".
+      { mDesAll. mAssertPure False; ss. iApply (pending1_unique with "A A2"). }
+      steps. mDesAll. des. subst.
+      mAssert _ with "INVS".
+      { iApply (initial_map_initialize with "INVS"). }
+      mUpd "A". mDesAll.
+      harg_tgt.
+      { iModIntro. iFrame. iSplits; et. xtra. }
+      steps.
+      (*** calling APC ***)
+      hAPC _.
+      { iIntros "A"; iDes. iSplitR "A".
+        { iLeft. iExists _, _. iFrame. iSplits; eauto. }
+        { iApply "A". }
+      }
+      { auto. }
+      fold wf. steps.
+      hret _; ss.
+      { iModIntro.
+        iDestruct "Q" as "[CLOSED %]". subst. iFrame.
+        iDestruct "FR" as "[H0 H1]". iDestruct "H0" as "[H0 | H0]".
+        { iDestruct "H0" as (f0 sz0) "[[[% H2] H3] H4]". des; subst.
+          iFrame. iSplits; auto.
+          iLeft. iExists _, _. iFrame. iPureIntro. eauto.
+        }
+        { iDes. des; subst. iSplitR "H1"; eauto. }
+      }
+      { iDestruct "Q" as "[_ %]". des; subst. iPureIntro.
+        rr. esplits; eauto.
+      }
+    }
+    econs; ss.
+    {
+      init.
+      rename mp_tgt into mpr_tgt.
+      assert(exists mp_src mp_tgt (mr_src mr_tgt: Σ),
+                mrp_src = Any.pair mp_src mr_src↑ ∧ mpr_tgt = Any.pair mp_tgt mr_tgt↑).
+      { inv WF. esplits; et. } des; clarify.
+      (*** init ***)
       unfold MapM.getF, MapA.getF, ccallU, ccallN.
       harg. fold wf. destruct x. ss.
       mDesAll; des; clarify.
       mDesOr "INVS".
-      2:{ mAssertPure False; ss. iApply (initial_map_no_points_to with "INVS A1"). }
+      2:{ mDesAll. mAssertPure False; ss. iApply (initial_map_no_points_to with "INVS A1"). }
       mDesAll. des; subst.
-      mAssertPure (0 ≤ n < a0)%Z.
+      mAssertPure (0 ≤ z < a0)%Z.
       { iApply (unallocated_range with "A2 A1"); eauto. }
+      mAssertPure _.
+      { iApply (black_map_get with "A3 A1"). }
+      subst. steps.
       harg_tgt.
       { iModIntro. iFrame. iSplits; et. xtra. }
       steps. force_r; auto. steps.
       (*** calling APC ***)
-      hAPC _; try assumption.
+      hAPC _.
       { iIntros "A"; iDes. iSplitR "A2".
         { iLeft. iExists _, _. iFrame. iSplits; auto. }
         { iApply "A2". }
       }
       { auto. }
-      fold wf. steps. s
-
-
-astop.
-
-r in WLE. des_ifs. astart 1. astep "Map.new" (([]: list val)↑). stb_tac. clarify.
-
-
-
-
-    {
-      (*** init ***)
-      init.
-      rename mp_tgt into mpr_tgt.
-      assert(exists mp_src mp_tgt (mr_src mr_tgt: Σ),
-                mrp_src = Any.pair mp_src mr_src↑ ∧ mpr_tgt = Any.pair mp_tgt mr_tgt↑).
-      { inv WF. esplits; et. } des; clarify.
-      (*** init ***)
-
-      unfold MapM.initF, MapA.initF, ccallU, ccallN.
-
-      harg. fold wf.
-      mDesAll; des; clarify.
-      mDesOr "INVS".
-      { mDesAll. des; subst. mAssertPure False; ss.
-        unfold pending. iDestruct "A1" as "[H0 H1]".
-        iApply (pending1_unique with "A H1").
+      fold wf. steps.
+      hret _; ss.
+      { iModIntro.
+        iDestruct "Q" as "[CLOSED %]". subst. iFrame.
+        iDestruct "FR" as "[H0 H1]". iDestruct "H0" as "[H0 | H0]".
+        2:{ iDes. iPoseProof (initial_map_no_points_to with "H0 H1") as "H"; ss. }
+        iDestruct "H0" as (f0 sz0) "[[[% H2] H3] H4]". des; subst.
+        iFrame. iSplits; auto.
+        iLeft. iExists _, _. iFrame. iPureIntro. eauto.
       }
-      unfold pending in ACC. mDesAll. steps.
-      harg_tgt.
-      { iModIntro. iFrame. iSplits; et. xtra. }
-      steps.
-      (*** calling APC ***)
-      hAPC _; try assumption.
-      { iIntros "A"; iDes. iSplitL "A".
-        - iRight. iLeft. iSplits; et.
-        - xtra.
+      { iDestruct "Q" as "[_ %]". subst. iPureIntro.
+        rr. esplits; eauto.
       }
-      fold wf. steps. r in WLE. des_ifs. astart 1. astep "Map.new" (([]: list val)↑). stb_tac. clarify.
-
-
-        (*** calling Map.new ***)
-        hcall _ _.
-        {
-          iDes; ss; des; clarify.
-          { iExFalso. iApply (mw_stateX_false with "INIT"); et. }
-          iModIntro. iSplits; ss. iSplitL "A".
-          { xtra. }
-          { iRight. iRight. iSplits; ss; et. iFrame. }
-        }
-        { esplits; ss; et. }
-        fold wf. steps. astop. steps. mDesAll; des; clarify. r in WLE0. des_ifs.
-        force_l; stb_tac; ss; clarify. steps.
-
-        hpost_tgt.
-        { iModIntro. iFrame. iSplits; ss.
-          iAssert ({{"LOCKED": ∃ f : Z → option Z,
-                 ((OwnM (mw_state f) ** OwnM (mw_stateX f)) ** ⌜mp_src0 = Any.upcast f⌝) **
-                 ⌜Some (Any.upcast (λ _ : Z, None), Any.upcast tt) = Some (mp_src0, mp_tgt0)⌝}})%I
-            with "[INV]" as "INV".
-          { iDes; ss. iSplits; ss; et. iFrame. }
-          xtra.
-        }
-        fold wf. steps. stb_tac; ss; clarify. steps. hide_k.
-
-
-
-        (*** calling App.init ***)
-        hcall _ _.
-        { iDes; ss; des; clarify. apply Any.upcast_inj in H10. des; clarify. clear_fast.
-          iModIntro. iSplits; ss; et.
-          iSplitR "LOCKED A A0"; cycle 1.
-          { iFrame. iSplits; ss; et. }
-          iSplitR.
-          { instantiate (1:=True%I); ss. }
-          iLeft. iSplits; ss; et. iFrame.
-        }
-        { i. iIntros "H". ss. iDes; des; clarify. }
-        unhide_k. steps. fold wf. mDesAll. des; clarify.
-
-
-
-        hpost_tgt.
-        { iModIntro. iSplits; ss; et. iFrame. iSplits; ss; et. xtra. }
-        fold wf. steps. force_l; stb_tac; ss; clarify. steps.
-        stb_tac; clarify.
-
-
-
-        (*** calling loop ***)
-        Opaque Z.eq_dec.
-        hcall _ _.
-        { iDes; ss; des; clarify; cycle 1.
-          { iExFalso. iApply (mw_state_false with "A2"); et. }
-          iModIntro. iSplits; ss; et. iSplitR "A A0 FR"; cycle 1.
-          { iSplits; ss; et. iFrame. iSplits; ss; et. }
-          iSplitR.
-          { instantiate (1:=True%I); ss. }
-          iLeft. iSplits; ss; et. iFrame.
-        }
-        { i. iIntros "H". ss. iDes. des; clarify. }
-        steps. fold wf. mDesAll. des; clarify.
-
-        hpost_tgt.
-        { iModIntro. iSplits; ss; et. iFrame. iSplits; ss; et. xtra. }
-        steps. fold wf.
-
-
-        (*** returning ***)
-        hret None; ss.
-        { iModIntro. iDes; ss; clarify; cycle 1.
-          { iExFalso. iApply (mw_state_false with "A"); et. }
-          iFrame.
-          iSplitL; cycle 1.
-          { iSplits; ss; et. }
-          iLeft. iSplits; ss; et. iFrame.
-        }
-        { iDes. clarify. iPureIntro. clarify. r. fold wf in WF0. exists None; esplits; et. }
-      }
-      { (* LOCKED *) mAssertPure False; ss. iApply (mw_stateX_false with "A1"); et. }
-    }
-
-
-
-    econs.
-    {
-      (*** init ***)
-      init.
-      rename mp_tgt into mpr_tgt.
-      assert(exists mp_src mp_tgt (mr_src mr_tgt: Σ),
-                mrp_src = Any.pair mp_src mr_src↑ ∧ mpr_tgt = Any.pair mp_tgt mr_tgt↑).
-      { inv WF. esplits; et. } des; clarify.
-      (*** init ***)
-
-      unfold loopF, MWC2.loopF, ccallU, ccallN.
-
-      harg. fold wf. mDesAll; des; clarify.
-      mDesOr "INVS"; mDesAll; des; clarify; steps.
-      { (* INIT *)
-        force_l; stb_tac; ss; clarify. steps.
-        harg_tgt.
-        { iModIntro. iFrame. iSplits; et. xtra. }
-        steps. stb_tac; ss; clarify.
-
-        hcall _ _.
-        { iDes. iModIntro. iFrame. iSplits; ss; et. iSplitR.
-          { instantiate (1:=True%I); ss. }
-          iLeft. iSplits; ss; et. iFrame.
-        }
-        { i. iIntros "H". ss. iDes; des; clarify. }
-        fold wf. steps. mDesAll; des; clarify. force_l; stb_tac; ss; clarify. steps.
-
-
-        hpost_tgt.
-        { iModIntro. iFrame. iSplits; ss; et. xtra. }
-        fold wf. steps. stb_tac; ss; clarify.
-
-
-        hcall _ _.
-        { iDes; ss; cycle 1.
-          { iExFalso. iApply (mw_state_false with "A2"); et. }
-          iModIntro. iFrame. iSplits; ss; et. iSplitR.
-          { instantiate (1:=True%I); ss. }
-          iLeft. iSplits; ss; et. iFrame.
-        }
-        { i. iIntros "H". ss. iDes. des; clarify. }
-        fold wf. steps. mDesAll; des; clarify. rewrite Any.upcast_downcast in *. clarify.
-
-        hpost_tgt.
-        { iModIntro. iFrame. iSplits ;ss; et. xtra. }
-        fold wf. steps.
-
-
-        hret None; ss.
-        { iDes; ss; clarify; cycle 1.
-          { iExFalso. iApply (mw_state_false with "A"); et. }
-          iModIntro. iSplits; ss; et. iFrame. iSplits; ss; et. iLeft. iSplits; ss; et. iFrame.
-        }
-        { iDes. clarify. iPureIntro. clarify. r. fold wf in WF0. exists None; esplits; et. }
-      }
-      mDesOr "INVS"; mDesAll; des; clarify; steps.
-      { (* UNINIT *) mAssertPure False; ss. iApply (mw_state_false with "A1"); et. }
-      { (* LOCKED *) mAssertPure False; ss. iApply (mw_state_false with "A1"); et. }
-    }
-
-
-    econs.
-    {
-      (*** init ***)
-      init.
-      rename mp_tgt into mpr_tgt.
-      assert(exists mp_src mp_tgt (mr_src mr_tgt: Σ),
-                mrp_src = Any.pair mp_src mr_src↑ ∧ mpr_tgt = Any.pair mp_tgt mr_tgt↑).
-      { inv WF. esplits; et. } des; clarify.
-      (*** init ***)
-
-      unfold putF, MWC2.putF, ccallU, ccallN.
-
-      harg. fold wf. mDesAll; ss; des; clarify. des_ifs_safe; ss. mDesAll; des; ss; clarify.
-      mDesOr "INVS".
-      { (* INIT *)
-        mDesAll; des; clarify.
-        mAssertPure (o = a).
-        { iApply (mw_state_eq with "A1"). iFrame. }
-        subst. rename a into full.
-        steps.
-        rename a2 into lst0. rename z0 into k. rename z into v.
-        change (λ k1 : Z, if dec k k1 then Some v else full k1) with (add k v full).
-        harg_tgt.
-        { iPoseProof ((mw_state_upd _ _ (add k v full)) with "A1 INIT") as "B".
-          iMod "B". iModIntro. iFrame. iSplits; ss; et. xtra. }
-        fold wf. steps. force_r; ss. steps.
-        destruct (dec (lst_cls lst0 k) uninit).
-        - steps.
-          unfold set. destruct (dec k k); ss. destruct x; steps.
-          + hAPC _; ss.
-            { iIntros "H"; iDes. iSplitL "A A0".
-              - iRight. iRight. iSplits; et. iFrame.
-              - iAssumption.
-            }
-            steps. fold wf. r in WLE. des_ifs. rewrite _UNWRAPU. steps.
-
-
-            hret None; ss.
-            { iDes; ss; clarify. apply Any.upcast_inj in H6. des; clarify.
-              iModIntro. iFrame. iSplits; ss; et. iLeft. iSplits; ss; et.
-              { iFrame. iAssumption. }
-              clear - PURE. iPureIntro. r. r in PURE. ss. i. specialize (PURE k0 v0). des_ifs; et.
-            }
-            { iDes; des; clarify. iPureIntro. r. fold wf in WF0. exists None; esplits; et. }
-          + steps.
-            astart 1. astep "Map.update" ([lst_map lst0; Vint k; Vint v]↑). stb_tac; ss; clarify.
-            hcall _ (Some (_, _)).
-            { iDes; clarify. instantiate (2:=(_, _, _, _)). cbn. iModIntro. iSplits; ss; et. iFrame.
-              iSplitL.
-              - iSplitR. { instantiate (1:=True%I); ss. } iRight. iRight. iSplits; ss; et. iSplitL "A"; ss.
-              - instantiate (1:=k). iSplits; ss; et. rewrite PURE2; ss.
-            }
-            { i. iIntros "H". ss. }
-            fold wf. mDesAll; des; clarify. steps. astop. steps.
-
-            hpost_tgt.
-            { iModIntro. iFrame. iSplits; ss. xtra. }
-            steps. fold wf. ss. des_ifs. rewrite _UNWRAPU. steps.
-            hret None; ss.
-            { iDes; ss; clarify. iModIntro. iSplits; ss; et. apply Any.upcast_inj in H6. des; clarify.
-              iSplitR "A A1"; ss; et.
-              - iLeft. iSplits; ss; et; iFrame.
-                clear - PURE. iPureIntro. r. r in PURE. ss. i. specialize (PURE k0 v0). des_ifs; et.
-              - iFrame. iSplits; ss; et.
-            }
-            { iDes; des; clarify. iPureIntro. r. fold wf in WF0. exists None; esplits; et. }
-        - steps.
-          destruct (lst_cls lst0 k) eqn:T; ss.
-          + steps. hAPC _; ss.
-            { iIntros "H"; iDes. iSplitL "A A0".
-              - iRight. iRight. iSplits; et. iFrame.
-              - iAssumption.
-            }
-            steps. fold wf. r in WLE. des_ifs. rewrite _UNWRAPU. steps.
-
-
-            hret None; ss.
-            { iDes; ss; clarify. apply Any.upcast_inj in H6. des; clarify.
-              iModIntro. iFrame. iSplits; ss; et. iLeft. iSplits; ss; et.
-              { iFrame. iAssumption. }
-              clear - T PURE. iPureIntro. r. r in PURE. ss. i. specialize (PURE k0 v0). unfold set.
-              des_ifs; et; try congruence.
-            }
-            { iDes; des; clarify. iPureIntro. r. fold wf in WF0. exists None; esplits; et. }
-          + steps.
-            astart 1. astep "Map.update" ([lst_map lst0; Vint k; Vint v]↑). stb_tac; ss; clarify.
-            hcall _ (Some (_, _)).
-            { iDes; clarify. instantiate (2:=(_, _, _, _)). cbn. iModIntro. iSplits; ss; et. iFrame.
-              iSplitL.
-              - iSplitR. { instantiate (1:=True%I); ss. } iRight. iRight. iSplits; ss; et. iSplitL "A"; ss.
-              - instantiate (1:=k). iSplits; ss; et. rewrite PURE2; ss.
-            }
-            { i. iIntros "H". ss. }
-            fold wf. mDesAll; des; clarify. steps. astop. steps.
-
-            hpost_tgt.
-            { iModIntro. iFrame. iSplits; ss. iCombine "A1" "INV" as "A". iAssumption. }
-            steps. fold wf. ss. des_ifs. rewrite _UNWRAPU. steps.
-            hret None; ss.
-            { iDes; ss; clarify. iModIntro. iSplits; ss; et. apply Any.upcast_inj in H6. des; clarify.
-              iSplitR "A A1"; ss; et.
-              - iLeft. iSplits; ss; et; iFrame.
-                clear - T PURE. iPureIntro. r. r in PURE. ss. i. specialize (PURE k0 v0).
-                des_ifs; et; try congruence.
-              - iFrame. iSplits; ss; et.
-            }
-            { iDes; des; clarify. iPureIntro. r. fold wf in WF0. exists None; esplits; et. }
-      }
-      mDesOr "INVS"; mDesAll; des; clarify.
-      { (* UNINIT *) mAssertPure False; ss. iApply (mw_state_false with "A1"); et. }
-      { (* LOCKED *) mAssertPure False; ss. iApply (mw_state_false with "A1"); et. }
-    }
-
-    econs.
-    {
-      (*** init ***)
-      init.
-      rename mp_tgt into mpr_tgt.
-      assert(exists mp_src mp_tgt (mr_src mr_tgt: Σ),
-                mrp_src = Any.pair mp_src mr_src↑ ∧ mpr_tgt = Any.pair mp_tgt mr_tgt↑).
-      { inv WF. esplits; et. } des; clarify.
-      (*** init ***)
-
-      unfold getF, MWC2.getF, ccallU, ccallN.
-
-      harg. fold wf. mDesAll; ss; des; clarify. des_ifs_safe; ss. mDesAll; des; ss; clarify.
-      mDesOr "INVS".
-      { (* INIT *)
-        mDesAll; des; clarify.
-        mAssertPure (o = a).
-        { iApply (mw_state_eq with "A1"). iFrame. }
-        subst. rename a into full.
-        steps.
-        rename a2 into lst0. rename z0 into k. rename z into v.
-        rewrite PURE1. steps.
-
-        harg_tgt.
-        { iModIntro. iFrame. iSplits; ss; et. xtra. }
-        steps. fold wf. force_r; ss. steps. force_r.
-        { exploit PURE; et. i. des_ifs. }
-        steps.
-        des_ifs.
-        - steps. hAPC (Some (_, _)); ss.
-          { iIntros "[A [B C]]". iSplitR "A"; try iAssumption. iRight. iRight. iSplits; ss; et. iFrame. }
-          fold wf. steps.
-          assert(T: lst_opt lst0 k = (Vint v)).
-          { r in PURE. exploit PURE; et. i; des_ifs. }
-          rewrite T. steps. rewrite _UNWRAPU. steps.
-          hret None; ss.
-          { iDes; ss; clarify. iModIntro. apply Any.upcast_inj in H6. des; clarify. iFrame. iSplits; ss; et.
-            iLeft. iSplits; ss; et. { iFrame. } }
-          { iDes; des; clarify. iPureIntro. r. fold wf in WF0. exists None; esplits; et. }
-        - steps. astart 1. astep "Map.access" ([lst_map lst0; Vint k]↑). stb_tac; ss; clarify.
-          hcall _ (Some (_, _)).
-          { iDes; clarify. instantiate (2:=(_, _, _, _)). cbn. iModIntro. iSplits; ss; et. iFrame.
-            des; clarify. apply Any.upcast_inj in H5. des; clarify.
-            iSplitL.
-            - iSplitR. { instantiate (1:=True%I); ss. } iRight. iRight. iSplits; ss; et.
-              iDestruct "A" as "[A B]". iFrame.
-            - iSplits; ss. { rewrite PURE2; ss. } iPureIntro. r in PURE. hexploit PURE; et. i; des_ifs. et. }
-          { i. iIntros "H". ss. }
-          fold wf. mDesAll; des; clarify. steps. astop. steps.
-
-          hpost_tgt.
-          { iModIntro. iFrame. iSplits; ss. iCombine "A1" "INV" as "A". iAssumption. }
-          steps. fold wf. ss. des_ifs. rewrite _UNWRAPU. steps.
-          hret None; ss.
-          { iDes; ss; clarify. iModIntro. iSplits; ss; et. apply Any.upcast_inj in H6. des; clarify.
-            iSplitR "A A1"; ss; et.
-            - iLeft. iSplits; ss; et; iFrame.
-            - iFrame. iSplits; ss; et. }
-          { iDes; des; clarify. iPureIntro. r. fold wf in WF0. exists None; esplits; et. }
-      }
-      mDesOr "INVS"; mDesAll; des; clarify.
-      { (* UNINIT *) mAssertPure False; ss. iApply (mw_state_false with "A1"); et. }
-      { (* LOCKED *) mAssertPure False; ss. iApply (mw_state_false with "A1"); et. }
     }
 
     econs; ss.
-  Unshelve. all: ss. all: try exact 0.
+    {
+      init.
+      rename mp_tgt into mpr_tgt.
+      assert(exists mp_src mp_tgt (mr_src mr_tgt: Σ),
+                mrp_src = Any.pair mp_src mr_src↑ ∧ mpr_tgt = Any.pair mp_tgt mr_tgt↑).
+      { inv WF. esplits; et. } des; clarify.
+      (*** init ***)
+      unfold MapM.setF, MapA.setF, ccallU, ccallN.
+      harg. fold wf. destruct x as [[? ?] ?]. ss.
+      mDesAll; des; clarify.
+      mDesOr "INVS".
+      2:{ mDesAll. mAssertPure False; ss. iApply (initial_map_no_points_to with "INVS A1"). }
+      mDesAll. des; subst.
+      mAssertPure (0 ≤ z < a0)%Z.
+      { iApply (unallocated_range with "A2 A1"); eauto. }
+      steps.
+      mAssert _ with "A3 A1".
+      { iApply (black_map_set with "A3 A1"). }
+      mUpd "A4". mDesAll.
+      harg_tgt.
+      { iModIntro. iFrame. iSplits; et. xtra. }
+      steps. force_r; auto. steps.
+      (*** calling APC ***)
+      hAPC _.
+      { iIntros "A"; iDes. iSplitR "A".
+        { iLeft. iExists _, _. iFrame. iSplits; eauto. }
+        { iApply "A". }
+      }
+      { auto. }
+      fold wf. steps.
+      hret _; ss.
+      { iModIntro.
+        iDestruct "Q" as "[CLOSED %]". subst. iFrame.
+        iDestruct "FR" as "[H0 H1]". iDestruct "H0" as "[H0 | H0]".
+        2:{ iDes. iPoseProof (initial_map_no_points_to with "H0 H1") as "H"; ss. }
+        iDestruct "H0" as (f0 sz0) "[[[% H2] H3] H4]". des; subst.
+        iFrame. iSplits; auto.
+        iLeft. iExists _, _. iFrame. iPureIntro. eauto.
+      }
+      { iDestruct "Q" as "[_ %]". subst. iPureIntro.
+        rr. esplits; eauto.
+      }
+    }
+    econs; ss.
+    {
+      init.
+      rename mp_tgt into mpr_tgt.
+      assert(exists mp_src mp_tgt (mr_src mr_tgt: Σ),
+                mrp_src = Any.pair mp_src mr_src↑ ∧ mpr_tgt = Any.pair mp_tgt mr_tgt↑).
+      { inv WF. esplits; et. } des; clarify.
+      (*** init ***)
+      unfold MapM.set_by_userF, MapA.set_by_userF, ccallU, ccallN.
+      harg. fold wf. destruct x. ss.
+      mDesOr "INVS".
+      2:{ mDesAll. mAssertPure False; ss. iApply (initial_map_no_points_to with "INVS A1"). }
+      mDesAll. des; subst. steps.
+      harg_tgt.
+      { iModIntro. iFrame. iSplits; et. xtra. }
+      steps. rewrite _UNWRAPU. rewrite STB_set. steps.
+      rewrite STB_setM in *. clarify. hcall _ _.
+      { instantiate (1:=(_, _, _)). ss. iModIntro.
+        iSplits; ss. iDes. iFrame. iSplits; ss; eauto.
+        { instantiate (1:=True%I). iSplit; ss. iLeft.
+          iExists _, _. iFrame. iPureIntro. eauto.
+        }
+      }
+      { i. ss. iIntros "H". iDes. subst. eauto. }
+      ss. mDesAll. subst.
+      hpost_tgt.
+      { iModIntro. iFrame. iSplits; ss; et. xtra. }
+      steps. hret _; ss.
+      { iModIntro.
+        iDestruct "Q" as "[CLOSED %]". subst. iFrame.
+        iDestruct "FR" as "[H0 H1]". iDestruct "H1" as "[H1 | H1]".
+        2:{ iDes. iPoseProof (initial_map_no_points_to with "H1 H0") as "H"; ss. }
+        iDestruct "H1" as (f0 sz0) "[[[% H2] H3] H4]". des; subst.
+        iSplitR "H0"; eauto. iLeft. iExists _, _. iFrame. iPureIntro. eauto.
+      }
+      { iDestruct "Q" as "[_ %]". subst. iPureIntro.
+        rr. esplits; eauto.
+      }
+    }
+    Unshelve. all: ss.
   Qed.
 
 End SIMMODSEM.
